Plausible/Chamelean/Enumerators.lean
@@ -196,9 +196,9 @@ instance : Enum (BitVec w) where
     To invoke this function, you will need to specify what type `α` is,
     for example by doing `runEnum (α := Nat) 10`. -/
 def runEnum [Enum α] (size : Nat) (limit : Nat := 10) : IO (List α) :=
-  return (LazyList.toList $ LazyList.take limit $ Enum.enum size)
+  return (LazyList.take limit $ Enum.enum size)
 
 /-- Samples from an `OptionT Enumerator` enumerator that is parameterized by its `size`,
     returning the enumerated list of `Option α` values (containing up to `limit` elements) in the `IO` monad -/
 def runSizedEnum (sizedEnum : Nat → OptionT Enumerator α) (size : Nat) (limit : Nat := 10) : IO (List (Option α)) :=
-  return (LazyList.toList $ LazyList.take limit $ (sizedEnum size) size)
+  return (LazyList.take limit $ (sizedEnum size) size)
